theories/language_commons.v
@@ -12,28 +12,3 @@ Inductive mixin_expr_class {val} :=
 
 Notation protocol val Σ :=
   (string -d> list val -d> (val -d> iPropO Σ) -d> iPropO Σ).
-
-Lemma excl_auth_eq A `{inG Σ (excl_authR (leibnizO A))} γ (x y: A):
-  own γ (◯E (x:leibnizO A)) -∗ own γ (●E (y:leibnizO A)) -∗ ⌜x = y⌝.
-Proof.
-  iIntros "H1 H2". iDestruct (own_op with "[$H1 $H2]") as "H".
-  iDestruct (own_valid with "H") as %HH%excl_auth_agree. done.
-Qed.
-
-Lemma excl_auth_upd `{!inG Σ (excl_authR (leibnizO A))} γ (x y z: A):
-  own γ (◯E (x:leibnizO A)) -∗ own γ (●E (y:leibnizO A)) ==∗
-  own γ (◯E (z:leibnizO A)) ∗ own γ (●E (z:leibnizO A)).
-Proof.
-  iIntros "H1 H2".
-  iDestruct (own_update_2 with "H1 H2") as ">[? ?]".
-  1: by apply excl_auth_update. iModIntro. iFrame.
-Qed.
-
-Lemma excl_auth_alloc A `{inG Σ (excl_authR (leibnizO A))} (x: A):
-  ⊢ |==> ∃ γ, own γ (◯E (x:leibnizO A)) ∗ own γ (●E (x:leibnizO A)).
-Proof.
-  iIntros.
-  iMod (own_alloc (●E (x:leibnizO A) ⋅ ◯E (x:leibnizO A))) as (γ) "[? ?]".
-  1: by apply excl_auth_valid. iModIntro. iExists _. iFrame.
-Qed.
-
